src/Common.v
@@ -30,4 +30,5 @@ Global Instance dec_eq_word : forall sz, DecidableEq (word sz) := weq.
 
 (* We want assign ranges of variables for certain purposes, so we need a total order,
    and we want S for to generate a fresh variable, so let's just use nat. *)
-Definition var := nat.
+Definition var := Z.
+Definition S := Z.succ.
